code/ecdsap256/Hacl.Impl.P256.ScalarMult.fsti
@@ -6,6 +6,7 @@ module ST = FStar.HyperStack.ST
 
 open Lib.IntTypes
 open Lib.Buffer
+open Lib.ByteSequence
 
 open Spec.P256
 open Spec.ECDSA
@@ -15,6 +16,17 @@ open Hacl.Impl.P256.Core
 
 open Spec.DH
 
+
+inline_for_extraction noextract
+val verifyQPrivate: 
+  pubKey: lbuffer uint8 (size 64) ->
+  Stack bool
+  (requires fun h -> live h pubKey)
+  (ensures  fun h0 r h1 -> modifies0 h0 h1 /\ (
+    let publicKeyX = nat_from_bytes_be (as_seq h1 (gsub pubKey (size 0) (size 32))) in 
+    let publicKeyY = nat_from_bytes_be (as_seq h1 (gsub pubKey (size 32) (size 32))) in
+    let pkJ = Spec.P256.toJacobianCoordinates (publicKeyX, publicKeyY) in 
+    r == not (verifyQValidCurvePointSpec pkJ)))
 
 inline_for_extraction noextract
 val ecp256scalar_mult:
